Safety commit for CPS transform work

src/D_cps_transform.lean
@@ -1,30 +1,32 @@
 import tactic.induction
 import tactic.ring_exp  -- for split_ifs
 
-def var_t := string
+set_option pp.generalized_field_notation false
 
 inductive term
--- | const : ℕ → term
-| var : var_t → term  -- TODO: use de Bruijn indexing to avoid the shadowing madness
-| lam : var_t → term → term
+| var : ℕ → term
+| lam : term → term
 | app : term → term → term
 
 namespace term
 def repr : term → string
--- | (const c) := nat.repr c
-| (var s) := s
-| (lam x b) := "(λ" ++ x ++ ", " ++ repr b ++ ")"
+| (var n) := nat.repr n
+| (lam b) := "(λ. " ++ repr b ++ ")"
 | (app f x) := "(" ++ repr f ++ " " ++ repr x ++ ")"
 
 instance : has_repr term := {repr := repr}
 
+def incr_indices : term → term
+| (var n) := var (n + 1)
+| (lam b) := lam (incr_indices b)
+| (app f x) := app (incr_indices f) (incr_indices x)
+
 def cps_transform : term → term
--- | (const n) := const n
-| (var x) := var x
-| (lam x b) := lam x (lam "k" (match cps_transform b with
-                               | (app f x) := app (app f x) (var "k")
-                               | t := app (var "k") t
-                               end))
+| (var n) := var n
+| (lam b) := lam (lam (match incr_indices (cps_transform b) with
+                       | (app f x) := app (app f x) (var 0)
+                       | t := app (var 0) t
+                       end))
 -- Lean isn't able to prove these recursive calls well-founded if they're in a
 -- match expression, so we have to do all pattern matching at top level
 | (app f (app g y)) := app (app (cps_transform g) (cps_transform y))
@@ -39,15 +41,20 @@ This takes the place of a match expression that would look like:
   end
 -/
 def cps_transform_cps_match_helper {α : Sort _} : term → (term → α) → α
-| (app f x) k := k (app (app f x) (var "k"))
-| t k := k (app (var "k") t)
+| (app f x) k := k (app (app f x) (var 0))
+| t k := k (app (var 0) t)
+
+def incr_indices_cps {α : Sort _} : term → (term → α) → α
+| (var n) k := k (var (n + 1))
+| (lam b) k := incr_indices_cps b (λb', k (lam b'))
+| (app f x) k := incr_indices_cps f (λf', incr_indices_cps x (λx', k (app f' x')))
 
 def cps_transform_cps {α : Sort _} : term → (term → α) → α
--- | (const n) := const n
 | (var x) k := k (var x)
-| (lam x b) k := cps_transform_cps b (λb',
-                   cps_transform_cps_match_helper b' (λl',
-                     k (lam x (lam "k" (l')))))
+| (lam b) k := cps_transform_cps b (λb',
+                 incr_indices_cps b' (λb'',
+                   cps_transform_cps_match_helper b'' (λl',
+                     k (lam (lam l')))))
 -- Lean isn't able to prove these recursive calls well-founded if they're in a
 -- match expression, so we have to do all pattern matching at top level
 | (app f (app g y)) k := cps_transform_cps g (λg',
@@ -58,27 +65,194 @@ def cps_transform_cps {α : Sort _} : term → (term → α) → α
                    cps_transform_cps x (λx',
                      k (app f' x')))
 
--- TODO: define an eval function, then prove the CPS transform correct
--- def subst (v : var_t)
--- | (var s) := s
+-- Helper function for variable binding
+-- The parameter is the variable to substitute in; the next argument is the
+-- current binder depth (initially 0); and the last argument is the term into
+-- which we're substituting
+-- TODO: do we need to worry about de Bruijn indices here?
+def subst_helper (vval : term) : ℕ → term → term
+| vid (var n) := if n = vid then vval else var n
+| vid (lam b) := lam (subst_helper (vid + 1) b)
+| vid (app f g) := app (subst_helper vid f) (subst_helper vid g)
 
-def subst (vname : var_t) (vval : term) : term → term
-| (var x) := if x = vname then vval else var x
-| (lam x b) := if x = vname then lam x b else lam x (subst b)
-| (app f g) := app (subst f) (subst g)
+-- Substitutes the first argument as (var 0) of the second (i.e., this assumes
+-- that the second argument is the *body* of some lambda -- do not include the
+-- outermost binder!)
+def subst : term → term → term := (λt, subst_helper t 0)
 
-#eval subst "x" (var "oops") (lam "y" (app (lam "q" (var "x")) (lam "x" (lam "x" (var "x")))))
+#eval lam (lam (app (lam (var 2)) (lam (lam (var 0)))))
+#eval subst (var 42) (lam (app (lam (var 2)) (lam (lam (var 0)))))
 
 inductive step : term → term → Prop
-| app {x v b} : step (app (lam v b) x) (subst v x b)
+| app {x b} : step (app (lam b) x) (subst x b)
+
+-- For testing:
+def eval : term → term
+| (app (lam b) x) := (subst x b)
+| x := x
 
 def is_value (t : term) := ¬∃(t' : term), step t t'
-def id_term := lam "x" (var "x")
+def id_term := lam (var 0)
 
 #eval cps_transform (id_term)
 
-lemma transform_spec : ∀ (t : term) (t' : term) (ht' : is_value t'), 
-  step t t' → step (app (cps_transform t) id_term) t' :=
+-- We first prove some auxiliary lemmas about helper functions
+lemma incr_indices_cps_equiv_incr_indices {α : Sort _} :
+  ∀ (t : term) (k : term → α), incr_indices_cps t k = k (incr_indices t) :=
+begin
+  intros t k,
+  induction' t,
+  case var { refl, },
+  case lam {
+    rw [incr_indices_cps, ih],
+    refl,
+  },
+  case app : f x ihf ihx {
+    rw [incr_indices_cps, ihf, ihx],
+    refl,
+  }
+end
+lemma match_helper_cps_equiv_match {α : Sort _} :
+  ∀ (t : term) (k : term → α),
+    cps_transform_cps_match_helper t k = k (cps_transform._match_1 t) :=
+begin
+  intros t k,
+  cases' t; refl,
+end
+
+-- Then prove that the CPS and non-CPS versions of the transform are equivalent
+-- (Because Lean's well-foundedness checker *really* doesn't like strong
+-- structural induction, we rely on term mode and its pattern-matching as much
+-- as possible here)
+lemma cps_transform_cps_equiv_cps_transform {α : Sort _} :
+  ∀ (t : term) (k : term → α), cps_transform_cps t k = k (cps_transform t)
+| (var n) k := rfl
+| (lam b) k :=
+  begin
+    rw [cps_transform_cps,
+        (cps_transform_cps_equiv_cps_transform b),
+        incr_indices_cps_equiv_incr_indices,
+        match_helper_cps_equiv_match],
+    refl,
+  end
+| (app f (app g y)) k :=
+  begin
+    rw [cps_transform_cps,
+        cps_transform_cps_equiv_cps_transform g,
+        cps_transform_cps_equiv_cps_transform y,
+        cps_transform_cps_equiv_cps_transform f],
+    refl,
+  end
+| (app f (var n)) k :=
+  begin
+    rw [cps_transform_cps,
+        cps_transform_cps_equiv_cps_transform f,
+        cps_transform_cps_equiv_cps_transform (var n)],
+    refl,
+  end
+| (app f (lam b)) k :=
+  begin
+    rw [cps_transform_cps,
+        cps_transform_cps_equiv_cps_transform f,
+        cps_transform_cps_equiv_cps_transform (lam b)],
+    refl,
+  end
+
+-- A predicate enforcing the constraint that a term can only have de Bruijn
+-- indices matching the number of nested binders at any given depth (the ℕ
+-- parameter)
+inductive valid_vars_at_depth : ℕ → term → Prop
+| bound : valid_vars_at_depth 0 (lam (var 0))
+| lam {b : term} : valid_vars_at_depth 1 b → valid_vars_at_depth 0 (lam b)
+| app {f x : term} : valid_vars_at_depth 0 f →
+                     valid_vars_at_depth 0 x →
+                     valid_vars_at_depth 0 (app f x)
+
+-- For a top-level expression, asserts that all de Bruijn indices are valid
+def valid_vars := valid_vars_at_depth 0
+
+-- TODO: may need to prove that stepping preserves valid var indices
+-- (i.e., has_valid_var_indices t ∧ t => t' → has_valid_var_indices t')
+
+def not_free_var (t : term) := ¬∃n, t = var n
+-- Now we prove that the non-CPS transform does what it's supposed to
+-- FIX(ED...I think)ME: this spec isn't nearly good enough. We need to be able to use IHs
+-- about intermediate terms, so the var/lam cases need to say something useful
+-- lemma transform_spec : ∀ (t : term) (t' : term) (ht' : is_value t'), 
+--   step t t' → step (app (cps_transform t) id_term) t'
+-- Take 2 - New spec:
+#eval lam (lam (app (var 0) (var 1)))
+#eval subst (lam (var 0)) (lam (app (var 0) (var 1)))
+#eval (lam (app (var 0) (lam (var 0))))
+lemma transform_spec : ∀ (t : term)
+                         (ht : valid_vars t)
+                         (t' : term)
+                         (k : term), 
+  step (app k t) t' → step (app (cps_transform t) k) t'
+| (var n) ht t' k hstep := by cases' ht
+| (lam b) ht t' k hstep :=
+  begin
+    rw cps_transform,
+    cases' hstep,
+    cases' b,
+    {
+      rw cps_transform,
+      rw incr_indices,
+      rw cps_transform._match_1,
+      rw subst,
+      dsimp only,
+      cases' b_1,
+      {
+        rw subst_helper,
+        cases' m,
+        {
+          split_ifs,
+          {
+            have hn : n = 0 := begin
+              cases' ht,
+              refl,
+              cases' ht,
+            end,
+            rw hn,
+            unfold has_add.add,
+            dsimp only [nat.add],
+            have h : subst (lam (app (var 0) (var 1))) (lam (var 0)) = (lam (app (var 0) (lam (var 0)))) := begin
+              -- TODO: this
+              sorry,
+            end,
+            have hstep1 : step (app (lam (lam (app (var 0) (var 1)))) (lam (var 0))) (lam (app (var 0) (lam (var 0)))) := step.app,
+            -- TODO: something's not right...hstep1 doesn't step to the goal...
+          },
+          { apply false.elim (h rfl), }
+        }
+      }
+    }
+    /-
+    cases' (cps_transform b),
+    {
+      rw incr_indices,
+      rw cps_transform._match_1,
+      cases' hstep,
+      rw subst,
+      dsimp only,
+      cases' b_1,
+      {
+        rw subst_helper,
+        cases' m,
+        {
+          simp,
+          
+        }
+      }
+    },
+    apply transform_spec b,
+    -/
+  end
+| (app f (app g y)) ht t' k hstep :=
+  begin
+    rw cps_transform,
+  end
+/-
 begin
   intros t t' ht' hstep,
   unfold is_value at ht',
@@ -111,11 +285,21 @@ begin
   },
   case app : t1 t2 ih_t1 ih_t2 {
     cases' hstep,
+    cases' x,
+    {
+      rw cps_transform,
+      
+      -- TODO: maybe the IH goes here?
+      rw cps_transform,
+      rw (ih_t1),
+      rw cps_transform.incr_indices,
+    }
     -- Use an IH? IDK?
   }
 end
+-/
 
-def test := app (lam "x" (var "x")) (app (lam "y" (var "y")) ((lam "q" (var "q"))))
+def test := app (lam (var 0)) (app (lam (var 0)) ((lam (var 0))))
 
 def s := repr test
 
